src/PrimitiveDecoder/RealExecSpec.v
@@ -1,35 +1,14 @@
 Require Import Core.Core Core.Notations Lib ErrorWithWriter.
-From ExtLib.Structures Require Import Monad MonadWriter Monoid.
-From ExtLib.Data Require Import List Monads.OptionMonad.
-
-Import MonadNotation.
-Import ListNotations.
-
-Open Scope monad.
 
 Section Encoder.
 
-Existing Class Monoid.
-Existing Instance Monoid_list_app.
-
-Definition real_prim_encoder (td : TYPE_descriptor) (r : list Z) : errW1 asn_enc_rval :=
-  let r := map (Byte.repr) r in
-  der_write_tags td >>= fun x => tell r >>= fun _ => ret (encode (1 + encoded x)).
+Definition real_encoder := 
+  fun td (r : list Z) => let r := map (Byte.repr) r in primitive_encoder td r.
 
 End Encoder.
 
 Section Decoder.
 
-Definition bool_decoder (td : TYPE_descriptor) (ls : list byte) : option (byte * Z) :=
-    match ls with
-    | [] => None
-    | _ => ber_check_tag td ls >>=
-                        fun x => let c := tag_consumed x in 
-                              let e := tag_expected x in 
-                              if (Zlength ls - c <? e) || negb (e =? 1) 
-                              then None 
-                              else (hd_error (skipn (Z.to_nat c) ls)) 
-                                     >>= fun y => Some (y, c + 1)
-    end.
+Definition real_decoder := primitive_decoder.
 
 End Decoder.
